Refinery/Term/Extrinsic/Refinement/Wk/Relation.lean
@@ -1,0 +1,82 @@
+import Refinery.Term.Extrinsic.Refinement.Wk.Basic
+import Refinery.Term.Extrinsic.Refinement.Relation
+
+namespace Refinery
+
+namespace Term
+
+variable {φ : Type u} {α : Type v} {ε : Type w} [S : Signature φ α ε]
+
+instance DRWS.instWkCongrLetMove : WkCongr (LetMove (S := S)) where
+  uwk_congr {Γ Δ} ρ _ _ _ da db h := by cases h with
+    | let_op hΓ hf da db =>
+      apply DRWS.cast_eq
+        (.base (.let_op (hΓ.wk ρ) hf (da.wk (hΓ.rightWk ρ)) (db.wk ((hΓ.leftWk ρ).scons _))))
+      simp
+      simp [ren_ren, <-Nat.liftWk_comp, Nat.liftWk_comp_succ]
+    | let_let₁ hΓ hΓc da db dc =>
+      apply DRWS.cast_eq
+        (.base (.let_let₁ (hΓ.wk ρ) (hΓc.wk (hΓ.rightWk ρ)) (da.wk (hΓc.rightWk (hΓ.rightWk ρ)))
+        (db.wk ((hΓc.leftWk (hΓ.rightWk ρ)).scons _))
+        (dc.wk ((hΓ.leftWk ρ).scons _))))
+      simp
+      simp [ren_ren, <-Nat.liftWk_comp, Nat.liftWk_comp_succ]
+    | let_let₂ hΓ hΓc da db dc =>
+      apply DRWS.cast_eq
+        (.base (.let_let₂ (hΓ.wk ρ) (hΓc.wk (hΓ.rightWk ρ)) (da.wk (hΓc.rightWk (hΓ.rightWk ρ)))
+        (db.wk (((hΓc.leftWk (hΓ.rightWk ρ)).scons _).scons _))
+        (dc.wk ((hΓ.leftWk ρ).scons _))))
+      simp
+      simp [ren_ren, <-Nat.liftWk_comp, Nat.liftWk_comp_succ]
+      rfl
+    | let_case hΓ hΓc da db dc dd =>
+      apply DRWS.cast_eq
+        (.base (.let_case (hΓ.wk ρ) (hΓc.wk (hΓ.rightWk ρ)) (da.wk (hΓc.rightWk (hΓ.rightWk ρ)))
+        (db.wk ((hΓc.leftWk (hΓ.rightWk ρ)).scons _))
+        (dc.wk ((hΓc.leftWk (hΓ.rightWk ρ)).scons _))
+        (dd.wk ((hΓ.leftWk ρ).scons _))))
+      simp
+      simp [ren_ren, <-Nat.liftWk_comp, Nat.liftWk_comp_succ]
+    | let_abort hΓ da db =>
+      apply DRWS.cast_eq
+        (.base (.let_abort (hΓ.wk ρ) (da.wk (hΓ.rightWk ρ)) (db.wk ((hΓ.leftWk ρ).scons _))))
+      simp
+      simp [ren_ren, <-Nat.liftWk_comp, Nat.liftWk_comp_succ]
+    | let_iter hΓ hΓc hcm hdm hcl hdl da db dc =>
+      apply DRWS.cast_eq
+        (.base (.let_iter (hΓ.wk ρ) (hΓc.wk (hΓ.rightWk ρ))
+        (hΓc.wkLeft_copy (hΓ.rightWk ρ))
+        (hΓc.wkLeft_del (hΓ.rightWk ρ))
+        (hΓ.wkLeft_copy ρ)
+        (hΓ.wkLeft_del ρ)
+        (da.wk ((hΓc.rightWk (hΓ.rightWk ρ))))
+        (db.wk (((hΓc.leftWk (hΓ.rightWk ρ)).scons _)))
+        (dc.wk ((hΓ.leftWk ρ).scons _))))
+      simp
+      simp [ren_ren, <-Nat.liftWk_comp, Nat.liftWk_comp_succ]
+
+instance DRWS.instWkCongrLetBind : WkCongr (LetBind (S := S)) where
+  uwk_congr {Γ Δ} ρ _ _ _ da db h := by cases h with
+    | bind_op hf da => apply DRWS.cast_eq (.base (.bind_op hf (da.wk ρ))) rfl rfl
+    | bind_let₂ hΓ da db =>
+      apply DRWS.cast_eq
+        (.base (.bind_let₂ (hΓ.wk ρ) (da.wk (hΓ.rightWk ρ))
+        (db.wk (((hΓ.leftWk ρ).scons _).scons _))))
+      simp
+      simp [ren_ren, <-Nat.liftWk_comp, Nat.liftWk_comp_succ]
+    | bind_case hΓ da db dc =>
+      apply DRWS.cast_eq
+        (.base (.bind_case (hΓ.wk ρ) (da.wk (hΓ.rightWk ρ))
+        (db.wk (((hΓ.leftWk ρ).scons _)))
+        (dc.wk (((hΓ.leftWk ρ).scons _)))))
+      simp
+      simp [ren_ren, <-Nat.liftWk_comp, Nat.liftWk_comp_succ]
+    | bind_iter hΓ hc hd da db =>
+      apply DRWS.cast_eq
+        (.base (.bind_iter (hΓ.wk ρ)
+        (hΓ.wkLeft_copy ρ)
+        (hΓ.wkLeft_del ρ)
+        (da.wk (hΓ.rightWk ρ))
+        (db.wk (((hΓ.leftWk ρ).scons _)))))
+      simp
+      simp [ren_ren, <-Nat.liftWk_comp, Nat.liftWk_comp_succ]
